add preservation package bridges

rocq/theories/TypeSystem/TypeSafetyClosureCleanupFrame.v
@@ -260,6 +260,139 @@ Definition eval_preserves_typing_roots_ready_prefix_mutual_statement : Prop :=
       store_no_shadow s' /\
       root_env_no_shadow R').
 
+Record typed_rooted_args_result
+    (env : global_env) (Ω : outlives_ctx) (s s' : store)
+    (vs : list value) (ps : list param) (Σ' : sctx)
+    (R' : root_env) (roots : list root_set) : Prop := {
+  typed_rooted_args_store_prefix : store_typed_prefix env s' Σ';
+  typed_rooted_args_values_types :
+    eval_args_values_have_types env Ω s' vs ps;
+  typed_rooted_args_refs_preserved : store_ref_targets_preserved env s s';
+  typed_rooted_args_roots : rooted_args_result R' s' roots vs
+}.
+
+Record typed_rooted_fields_result
+    (env : global_env) (s s' : store) (lts : list lifetime)
+    (args : list Ty) (values : list (string * value))
+    (defs : list field_def) (Σ' : sctx) (R' : root_env)
+    (roots : root_set) : Prop := {
+  typed_rooted_fields_store_prefix : store_typed_prefix env s' Σ';
+  typed_rooted_fields_values_types :
+    struct_fields_have_type env s' lts args values defs;
+  typed_rooted_fields_refs_preserved : store_ref_targets_preserved env s s';
+  typed_rooted_fields_roots : rooted_fields_result R' s' roots values
+}.
+
+Definition eval_preserves_typing_roots_ready_prefix_mutual_package_statement
+    : Prop :=
+  (forall env s e s' v,
+    eval env s e s' v ->
+    forall (Ω : outlives_ctx) (n : nat) R Σ T Σ' R' roots,
+      provenance_ready_expr e ->
+      store_typed_prefix env s Σ ->
+      store_roots_within R s ->
+      store_no_shadow s ->
+      root_env_no_shadow R ->
+      typed_env_roots env Ω n R Σ e T Σ' R' roots ->
+      typed_rooted_eval_result env s s' v T Σ' R' roots) /\
+  (forall env s args s' vs,
+    eval_args env s args s' vs ->
+    forall (Ω : outlives_ctx) (n : nat) R Σ ps Σ' R' roots,
+      provenance_ready_args args ->
+      store_typed_prefix env s Σ ->
+      store_roots_within R s ->
+      store_no_shadow s ->
+      root_env_no_shadow R ->
+      typed_args_roots env Ω n R Σ args ps Σ' R' roots ->
+      typed_rooted_args_result env Ω s s' vs ps Σ' R' roots) /\
+  (forall env s fields defs s' values,
+    eval_struct_fields env s fields defs s' values ->
+    forall (Ω : outlives_ctx) (n : nat) lts args R Σ Σ' R' roots,
+      provenance_ready_fields fields ->
+      store_typed_prefix env s Σ ->
+      store_roots_within R s ->
+      store_no_shadow s ->
+      root_env_no_shadow R ->
+      typed_fields_roots env Ω n lts args R Σ fields defs Σ' R' roots ->
+      typed_rooted_fields_result env s s' lts args values defs Σ' R' roots).
+
+Lemma eval_preserves_typing_roots_ready_prefix_mutual_statement_to_package :
+  eval_preserves_typing_roots_ready_prefix_mutual_statement ->
+  eval_preserves_typing_roots_ready_prefix_mutual_package_statement.
+Proof.
+  intros [Hexpr [Hargs Hfields]].
+  split.
+  - intros env_a st_a expr_a st_b val_a Heval Ω_a n_a R_a Σ_a T_a
+      Σ_b R_b roots_a Hprov Hprefix Hroots Hshadow Hrn Htyped.
+    destruct (Hexpr env_a st_a expr_a st_b val_a Heval Ω_a n_a R_a
+                Σ_a T_a Σ_b R_b roots_a
+                Hprov Hprefix Hroots Hshadow Hrn Htyped)
+      as [Hprefix' [Hv [Hpres [Hroots' [Hvroots [Hshadow' Hrn']]]]]].
+    constructor.
+    + exact Hprefix'.
+    + exact Hv.
+    + exact Hpres.
+    + constructor; assumption.
+  - split.
+    + intros env_a st_a args_a st_b vs_a Heval Ω_a n_a R_a Σ_a ps_a
+      Σ_b R_b roots_a Hprov Hprefix Hroots Hshadow Hrn Htyped.
+      destruct (Hargs env_a st_a args_a st_b vs_a Heval Ω_a n_a R_a Σ_a
+                  ps_a Σ_b R_b roots_a
+                  Hprov Hprefix Hroots Hshadow Hrn Htyped)
+        as [Hprefix' [Hvs [Hpres [Hroots' [Hvroots [Hshadow' Hrn']]]]]].
+      constructor.
+      * exact Hprefix'.
+      * exact Hvs.
+      * exact Hpres.
+      * constructor; assumption.
+    + intros env_a st_a fields_a defs_a st_b values_a Heval Ω_a n_a lts_a
+      ty_args_a R_a Σ_a Σ_b R_b roots_a Hprov Hprefix Hroots Hshadow
+      Hrn Htyped.
+      destruct (Hfields env_a st_a fields_a defs_a st_b values_a Heval Ω_a
+                  n_a lts_a ty_args_a R_a Σ_a Σ_b R_b roots_a Hprov
+                  Hprefix Hroots Hshadow Hrn Htyped)
+        as [Hprefix' [Hvalues [Hpres [Hroots' [Hvroots [Hshadow' Hrn']]]]]].
+      constructor.
+      * exact Hprefix'.
+      * exact Hvalues.
+      * exact Hpres.
+      * constructor; assumption.
+Qed.
+
+Lemma eval_preserves_typing_roots_ready_prefix_mutual_package_statement_to_plain :
+  eval_preserves_typing_roots_ready_prefix_mutual_package_statement ->
+  eval_preserves_typing_roots_ready_prefix_mutual_statement.
+Proof.
+  intros [Hexpr [Hargs Hfields]].
+  split.
+  - intros env_a st_a expr_a st_b val_a Heval Ω_a n_a R_a Σ_a T_a
+      Σ_b R_b roots_a Hprov Hprefix Hroots Hshadow Hrn Htyped.
+    destruct (Hexpr env_a st_a expr_a st_b val_a Heval Ω_a n_a R_a
+                Σ_a T_a Σ_b R_b roots_a
+                Hprov Hprefix Hroots Hshadow Hrn Htyped)
+      as [Hprefix' Hv Hpres Hrooted].
+    destruct Hrooted as [Hroots' Hvroots Hshadow' Hrn'].
+    repeat split; assumption.
+  - split.
+    + intros env_a st_a args_a st_b vs_a Heval Ω_a n_a R_a Σ_a ps_a
+      Σ_b R_b roots_a Hprov Hprefix Hroots Hshadow Hrn Htyped.
+      destruct (Hargs env_a st_a args_a st_b vs_a Heval Ω_a n_a R_a Σ_a
+                  ps_a Σ_b R_b roots_a
+                  Hprov Hprefix Hroots Hshadow Hrn Htyped)
+        as [Hprefix' Hvs Hpres Hrooted].
+      destruct Hrooted as [Hroots' Hvroots Hshadow' Hrn'].
+      repeat split; assumption.
+    + intros env_a st_a fields_a defs_a st_b values_a Heval Ω_a n_a lts_a
+      ty_args_a R_a Σ_a Σ_b R_b roots_a Hprov Hprefix Hroots Hshadow
+      Hrn Htyped.
+      destruct (Hfields env_a st_a fields_a defs_a st_b values_a Heval Ω_a
+                  n_a lts_a ty_args_a R_a Σ_a Σ_b R_b roots_a Hprov
+                  Hprefix Hroots Hshadow Hrn Htyped)
+        as [Hprefix' Hvalues Hpres Hrooted].
+      destruct Hrooted as [Hroots' Hvroots Hshadow' Hrn'].
+      repeat split; assumption.
+Qed.
+
 Definition eval_preserves_param_scope_roots_ready_mutual_statement : Prop :=
   (forall env s e s' v,
     eval env s e s' v ->
